Compiler/CompilerSimple.v
@@ -1,0 +1,94 @@
+Require Import Kami.Syntax Kami.Compiler.Compiler.
+Require Import Kami.Notations.
+
+Section Simple.
+
+  Variable ty : Kind -> Type.
+  Variable regMapTy : Type.
+
+  Inductive RmeSimple :=
+  | VarRME (v : regMapTy) : RmeSimple
+  | UpdRegRME (r : string)(pred : Bool @# ty)(k : FullKind)(val : Expr ty k)(regMap : RmeSimple) : RmeSimple
+  | WriteRME (idxNum num : nat) (writePort dataArray : string) (idx  : Bit (Nat.log2_up idxNum) @# ty) (Data : Kind)
+             (val : Array num Data @# ty)
+             (mask : option (Array num Bool @# ty)) (pred : Bool @# ty) (writeMap readMap : RmeSimple)
+             (arr : Array idxNum Data @# ty) : RmeSimple
+  | ReadReqRME (idxNum num : nat) (readReq readReg dataArray : string) (idx : Bit (Nat.log2_up idxNum) @# ty) (Data : Kind)
+               (isAddr : bool) (pred : Bool @# ty) (writeMap readMap : RmeSimple)
+               (arr : Array idxNum Data @# ty) : RmeSimple
+  | ReadRespRME (idxNum num : nat) (readResp readReg dataArray : string) (Data : Kind)
+               (isAddr : bool) (readMap : RmeSimple) : RmeSimple
+  | AsyncReadRME (idxNum num : nat) (readPort dataArray : string) (idx : Bit (Nat.log2_up idxNum) @# ty) (pred : Bool @# ty)
+                 (k : Kind)(readMap : RmeSimple) : RmeSimple
+  | CompactRME (regMap: RmeSimple): RmeSimple.
+
+  Fixpoint RmeSimple_of_RME(x : RegMapExpr ty regMapTy) : RmeSimple :=
+    match x with
+    | VarRegMap v => VarRME v
+    | UpdRegMap r pred k val regMap => UpdRegRME r pred val (RmeSimple_of_RME regMap)
+    | CompactRegMap x' => CompactRME (RmeSimple_of_RME x')
+    end.
+
+  Inductive CompActionSimple : Kind -> Type :=
+  | CompCall_simple (f : string)(argRetK : Kind * Kind)(pred : Bool @# ty)(arg : fst argRetK @# ty)
+                    lret (cont : fullType ty (SyntaxKind (snd argRetK)) -> CompActionSimple lret) : CompActionSimple lret
+  | CompLetExpr_simple k (e : Expr ty k) lret (cont : fullType ty k -> CompActionSimple lret) : CompActionSimple lret
+  | CompNondet_simple k lret (cont : fullType ty k -> CompActionSimple lret) : CompActionSimple lret
+  | CompSys_simple (pred: Bool @# ty) (ls: list (SysT ty)) lret (cont: CompActionSimple lret): CompActionSimple lret
+  | CompReadReg_simple (r: string) (k: FullKind) (readMap : RmeSimple) lret
+                       (cont: fullType ty k -> CompActionSimple lret): CompActionSimple lret
+  | CompRet_simple lret (e: lret @# ty) (newMap: RmeSimple) : CompActionSimple lret
+  | CompLetFull_simple k (a: CompActionSimple k) lret (cont: fullType ty (SyntaxKind k) ->
+                                                      regMapTy -> CompActionSimple lret): CompActionSimple lret
+  | CompAsyncRead_simple (idxNum num : nat) (readPort dataArray : string) (idx : Bit (Nat.log2_up idxNum) @# ty)
+                         (pred : Bool @# ty)
+                         (k : Kind)
+                         (readMap : RmeSimple) lret
+                         (cont : fullType ty (SyntaxKind (Array num k)) -> CompActionSimple lret) : CompActionSimple lret
+  | CompSyncReadRes_simple (idxNum num : nat) (readResp readReg dataArray : string) (Data : Kind) (isAddr : bool)
+                           (readMap : RmeSimple) lret
+                           (cont : fullType ty (SyntaxKind (Array num Data)) -> CompActionSimple lret) : CompActionSimple lret
+  | CompWrite_simple (idxNum : nat) (Data : Kind) (writePort dataArray : string) (readMap : RmeSimple) lret
+                     (cont : ty (Array idxNum Data) -> CompActionSimple lret) : CompActionSimple lret
+  | CompSyncReadReq_simple (idxNum num : nat) (Data : Kind) (readReq readReg dataArray : string) (isAddr : bool)
+                           (readMap : RmeSimple) lret
+                           (cont : ty (Array idxNum Data) -> CompActionSimple lret) : CompActionSimple lret.
+
+  Fixpoint CompActionSimple_of_CA{k}(a : CompActionT ty regMapTy k) : CompActionSimple k :=
+    match a with
+    | CompCall f argRetK pred arg lret cont => CompCall_simple f argRetK pred arg (fun x => CompActionSimple_of_CA (cont x))
+    | CompLetExpr k e lret cont => CompLetExpr_simple e (fun x => CompActionSimple_of_CA (cont x))
+    | CompNondet k lret cont => CompNondet_simple k (fun x => CompActionSimple_of_CA (cont x))
+    | CompSys pred ls lret cont => CompSys_simple pred ls (CompActionSimple_of_CA cont)
+    | CompRead r k readMap lret cont => CompReadReg_simple r k (RmeSimple_of_RME readMap)
+                                                           (fun x => CompActionSimple_of_CA (cont x))
+    | CompRet lret e newMap => CompRet_simple e (RmeSimple_of_RME newMap)
+    | CompLetFull k a lret cont => CompLetFull_simple (CompActionSimple_of_CA a) (fun x y => CompActionSimple_of_CA (cont x y))
+    | CompAsyncRead idxNum num readPort dataArray idx pred k readMap lret cont =>
+      CompLetFull_simple (CompRet_simple (($$WO)%kami_expr : Void @# ty)
+                                         (AsyncReadRME idxNum num readPort dataArray idx pred k (RmeSimple_of_RME readMap)))
+                         (fun _ y => CompAsyncRead_simple idxNum readPort dataArray idx pred (VarRME y)
+                                                          (fun arr => CompActionSimple_of_CA (cont arr)))
+    | CompWrite idxNum num writePort dataArray idx Data val mask pred writeMap readMap lret cont =>
+      @CompWrite_simple idxNum Data writePort dataArray (RmeSimple_of_RME readMap) lret
+                        (fun arr => 
+                           CompLetFull_simple (CompRet_simple (($$ WO)%kami_expr : Void @# ty)
+                                                              (@WriteRME idxNum num writePort dataArray idx Data val mask pred
+                                                                         (RmeSimple_of_RME writeMap)
+                                                                         (RmeSimple_of_RME readMap) (#arr)%kami_expr))
+                                              (fun _ y => CompActionSimple_of_CA (cont y)))
+    | CompSyncReadReq idxNum num readReq readReg dataArray idx Data isAddr pred writeMap readMap lret cont =>
+      @CompSyncReadReq_simple idxNum num Data readReq readReg dataArray isAddr (RmeSimple_of_RME readMap) lret
+                              (fun x => CompLetFull_simple (CompRet_simple (($$ WO)%kami_expr : Void @# ty)
+                                                                           (@ReadReqRME idxNum num readReq readReg dataArray
+                                                                                        idx Data isAddr pred
+                                                                                        (RmeSimple_of_RME writeMap)
+                                                                                        (RmeSimple_of_RME readMap)
+                                                                                        (#x)%kami_expr))
+                                                           (fun _ y => CompActionSimple_of_CA (cont y)))
+    | CompSyncReadRes idxNum num readResp readReg dataArray Data isAddr readMap lret cont =>
+      CompSyncReadRes_simple idxNum readResp readReg dataArray isAddr (@ReadRespRME idxNum num readResp readReg dataArray Data isAddr (RmeSimple_of_RME readMap))
+                             (fun x => CompActionSimple_of_CA (cont x))
+    end.
+
+End Simple.
