Compiler/CompilerSimpleProps.v
@@ -1,13 +1,13 @@
-Require Import Kami.All.
+Require Import Kami.Syntax Kami.PPlusProperties.
 Require Import Kami.Notations.
-Require Import Kami.CVSimpleSem.
-Require Import Kami.CVSimple.
-Require Import Kami.CVProperties.
-Require Import Kami.CompileVerifiable.
+Require Import Kami.Compiler.CompilerSimpleSem.
+Require Import Kami.Compiler.CompilerSimple.
+Require Import Kami.Compiler.CompilerProps.
+Require Import Kami.Compiler.Compiler.
 
 Lemma RME_Simple_RME_Equiv map:
   forall old upds,
-    Sem_RME_simple (RME_simple_of_RME map) (old, upds) ->
+    Sem_RmeSimple (RmeSimple_of_RME map) (old, upds) ->
     SemRegMapExpr map (old, upds).
 Proof.
   induction map; intros; try (inv H; EqDep_subst).
@@ -19,7 +19,7 @@ Qed.
 
 Lemma CA_Simple_CA_Equiv {k : Kind} (ca : CompActionT type (RegsT * list RegsT) k) :
   forall regMap calls val,
-    SemCA_simple (CA_simple_of_CA ca) regMap calls val ->
+    SemCompActionSimple (CompActionSimple_of_CA ca) regMap calls val ->
     SemCompActionT ca regMap calls val.
 Proof.
   induction ca; intros; try ((inv H0 || inv H); EqDep_subst).
@@ -32,13 +32,13 @@ Proof.
   - econstructor 7; eauto.
     destruct regMap; inv HRegMapWf; econstructor; eauto using RME_Simple_RME_Equiv.
   - econstructor 8; eauto.
-  - inv HSemCA_simple_a; simpl in *; EqDep_subst.
-    inv HSemCA_simple_cont; simpl in *; EqDep_subst.
+  - inv HSemCompActionSimple_a; simpl in *; EqDep_subst.
+    inv HSemCompActionSimple_cont; simpl in *; EqDep_subst.
     inv HRegMapWf; inv H0; EqDep_subst.
     inv HReadMap.
     econstructor 9; eauto using RME_Simple_RME_Equiv.
-  - inv HSemCA_simple; simpl in *; EqDep_subst; rewrite unifyWO in *.
-    inv HSemCA_simple_a; EqDep_subst.
+  - inv HSemCompActionSimple; simpl in *; EqDep_subst; rewrite unifyWO in *.
+    inv HSemCompActionSimple_a; EqDep_subst.
     destruct regMap_a; inv HRegMapWf; inv H0; EqDep_subst.
     + inv HUpdate; EqDep_subst.
       econstructor 10; eauto using RME_Simple_RME_Equiv.
@@ -49,13 +49,13 @@ Proof.
         eapply SemUpdRegMapFalse; eauto using RME_Simple_RME_Equiv.
     + econstructor 11; eauto using RME_Simple_RME_Equiv.
       econstructor; eauto using RME_Simple_RME_Equiv.
-  - inv HSemCA_simple; simpl in *; EqDep_subst; rewrite unifyWO in *.
-    inv HSemCA_simple_a; EqDep_subst.
+  - inv HSemCompActionSimple; simpl in *; EqDep_subst; rewrite unifyWO in *.
+    inv HSemCompActionSimple_a; EqDep_subst.
     destruct regMap_a; inv HRegMapWf; inv H0; EqDep_subst;[|discriminate].
     econstructor 12; eauto.
     econstructor; eauto using RME_Simple_RME_Equiv.
-  - inv HSemCA_simple; simpl in *; EqDep_subst; rewrite unifyWO in *.
-    inv HSemCA_simple_a; EqDep_subst.
+  - inv HSemCompActionSimple; simpl in *; EqDep_subst; rewrite unifyWO in *.
+    inv HSemCompActionSimple_a; EqDep_subst.
     destruct regMap_a; inv HRegMapWf; inv H0; EqDep_subst;[discriminate|].
     econstructor 13; eauto using RME_Simple_RME_Equiv.
     econstructor; eauto using RME_Simple_RME_Equiv.
@@ -69,20 +69,20 @@ Qed.
 
 Lemma CA_Simple_Trace_CA_Trace_Equiv (ca : RegsT -> CompActionT type (RegsT * list RegsT) Void) :
   forall regInits o lupds lcalls,
-    SemCA_simple_Trace regInits (fun s => CA_simple_of_CA (ca s)) o lupds lcalls ->
+    SemCompActionSimple_Trace regInits (fun s => CompActionSimple_of_CA (ca s)) o lupds lcalls ->
     SemCompTrace regInits ca o lupds lcalls.
 Proof.
   induction 1;[econstructor 1 | econstructor 2]; eauto using CA_Simple_CA_Equiv.
 Qed.
 
-Lemma CA_Simple_TraceEquiv (b : BaseModule) (lrf : list RegFileBase) o :
+Lemma CompActionSimpleTraceEquiv (b : BaseModule) (lrf : list RegFileBase) o :
   let m := inlineAll_All_mod (mergeSeparatedSingle b lrf) in
   let regInits := (getRegisters b) ++ (concat (map getRegFileRegisters lrf)) in
   forall rules lupds lcalls
          (HWfMod : WfMod (mergeSeparatedSingle b lrf))
          (HNoSelfCallsBase : NoSelfCallBaseModule b),
     SubList rules (getRules b) ->
-    SemCA_simple_Trace regInits (fun s => CA_simple_of_CA
+    SemCompActionSimple_Trace regInits (fun s => CompActionSimple_of_CA
                                             (compileRulesRf type (s, nil)
                                                             rules lrf)) o lupds lcalls ->
     (forall upds u, In upds lupds -> In u upds -> (NoDup (map fst u)) /\
